Use `receive_follow_up` in `repeated_receive_idempotency`

src/Thorn_Calculus-Semantics-Synchronous.thy
@@ -112,6 +112,14 @@ proof -
     unfolding receive_follow_up_def .
 qed
 
+abbreviation repeated_receive_follow_up :: "chan family \<Rightarrow> (val \<Rightarrow> process family) \<Rightarrow> nat \<Rightarrow> val family \<Rightarrow> process family" where
+  "repeated_receive_follow_up A \<P> n X \<equiv> receive_follow_up (\<lambda>v. \<P> v \<parallel> A \<triangleright>\<^sup>\<infinity> x. \<P> x) n X"
+
+lemma repeated_receive_follow_up_split:
+  shows "repeated_receive_follow_up A \<P> n X = receive_follow_up \<P> n X \<parallel> (A \<triangleright>\<^sup>\<infinity> x. \<P> x) \<guillemotleft> suffix n"
+  unfolding receive_follow_up_def and adapted_after_parallel
+  by fastforce
+
 inductive
   synchronous_transition :: "action \<Rightarrow> process family relation"
   (\<open>'(\<rightarrow>\<^sub>s\<lparr>_\<rparr>')\<close>)
